proofs/proofsystem/Unfold.v
@@ -338,8 +338,6 @@ Proof.
   subst. f_equal. apply term_rep_irrel.
 Qed.
 
-(*TODO: preds*)
-
 (*Get the function body and arguments for a funsym. We do in 2 parts, even though this
   is less efficient (should implement 1-pass version)*)
 Definition get_rec_fun_body_args (gamma: context) (f: funsym) :
@@ -814,3 +812,717 @@ Proof.
   apply check_sublist_prop in H; auto.
 Qed.
 
+(*Predicate symbol unfolding (can we reduce duplication?)*)
+
+Section FindPred.
+Variable p: predsym.
+(*NOTE: will need to go left to right - could substitute in terms that should
+  later be unfolded*)
+Fixpoint find_pred_app_t(t: term) : list (list vty * list term) :=
+  match t with 
+  | Tfun f1 tys tms => concat (map find_pred_app_t tms) 
+  | Tlet t1 x t2 => find_pred_app_t t1 ++ find_pred_app_t t2
+  | Tif f1 t1 t2 => find_pred_app_f f1 ++ find_pred_app_t t1 ++
+  find_pred_app_t t2 
+  | Tmatch t ty ps => find_pred_app_t t ++
+    concat (map (fun x => find_pred_app_t (snd x)) ps)
+  | Teps f1 x => find_pred_app_f f1
+  | _ => nil
+  end
+with find_pred_app_f (f1: formula) : list (list vty * list term) :=
+  match f1 with
+  | Fpred p1 tys tms => (if predsym_eq_dec p1 p then [(tys, tms)] else nil)
+  ++  concat (map find_pred_app_t tms)
+  | Fquant q x f1 => find_pred_app_f f1
+  | Fbinop p f1 f2 => find_pred_app_f f1 ++ find_pred_app_f f2
+  | Feq ty t1 t2 => find_pred_app_t t1 ++ find_pred_app_t t2
+  | Flet t x f1 => find_pred_app_t t ++ find_pred_app_f f1
+  | Fif f1 f2 f3 => find_pred_app_f f1 ++ find_pred_app_f f2 ++
+  find_pred_app_f f3
+  | Fmatch t ty ps => find_pred_app_t t ++
+    concat (map (fun x => find_pred_app_f (snd x)) ps)
+  | _ => nil
+  end.
+
+Definition sub_body_f (args: list vsymbol) (body: formula) tys tms :=
+  safe_sub_fs (combine (map (ty_subst_var (s_params p) tys) args) tms) 
+    (ty_subst_wf_fmla (s_params p) tys body).
+
+Definition sub_pred_body_f (args: list vsymbol) (body: formula) tys tms (f1: formula) :=
+  replace_fmla_f (Fpred p tys tms) (sub_body_f args body tys tms) f1.
+
+Definition unfold_p_single_aux (f1: formula) (args: list vsymbol) (body: formula)
+  (x: (list vty * list term)) :=
+  let tys := fst x in
+  let tms := snd x in
+  sub_pred_body_f args body tys tms f1.
+
+Definition unfold_p_aux (f1: formula) (args: list vsymbol) (body: formula) :=
+  fold_left (fun acc x =>
+    unfold_p_single_aux acc args body x) (find_pred_app_f f1) f1.
+  (* let apps := find_fun_app_f f1 in
+  fold_left (fun (acc: formula) x => let tys := fst x in
+    let tms := snd x in
+    sub_fun_body_f args body tys tms acc) apps f1.*)
+
+End FindPred.
+
+Lemma pred_defined_valid {gamma p args body}:
+  valid_context gamma ->
+  pred_defined gamma p args body ->
+  funpred_def_valid_type gamma (pred_def p args body).
+Proof.
+  unfold pred_defined.
+  intros gamma_valid p_in.
+  destruct p_in as [[fs [fs_in p_in]] | p_in].
+  - pose proof (funpred_def_valid gamma_valid _ fs_in).
+    unfold funpred_valid in H. destruct H as [Hval _].
+    rewrite Forall_forall in Hval; auto.
+  - pose proof (valid_context_defs _ gamma_valid).
+    rewrite Forall_forall in H. specialize (H _ p_in).
+    apply H.
+Qed.
+
+(*Almost the same proof as before, can we generalize?
+  Don't think so because [term_rep] and [formula_rep] are different*)
+Theorem sub_body_f_rep {gamma} (gamma_valid: valid_context gamma)
+  (p: predsym) (args: list vsymbol) (body: formula) 
+  (p_in: pred_defined gamma p args body)
+  (tms: list term) (tys: list vty)
+  (Hlenat: length args = length tms)
+  (Htysval: Forall (valid_type gamma) tys)
+  (pd: pi_dom) (pf: pi_funpred gamma_valid pd)
+  (pf_full: full_interp gamma_valid pd pf)
+  (vt: val_typevar) (vv: val_vars pd vt) Hty1 Hty2:
+  formula_rep gamma_valid pd vt pf vv (sub_body_f p args body tys tms) Hty1 =
+  formula_rep gamma_valid pd vt pf vv (Fpred p tys tms) Hty2.
+Proof.
+  (*Get some info from typing*)
+  pose proof (pred_defined_valid gamma_valid p_in) as Hdef.
+  simpl in Hdef.
+  destruct Hdef as [Htyb [Hfvargs [Hsubvars [Hnargs Hargs]]]].
+  (*First, simplify RHS*)
+  simpl_rep_full.
+  destruct pf_full as [_ [Hpreds _]].
+  assert (Hlen: length tys = length (s_params p)). {
+    inversion Hty2; subst; auto.
+  }
+  assert (Hmaplen: length (map (v_subst vt) tys) = length (s_params p)). {
+    rewrite map_length; auto.
+  }
+  rewrite (Hpreds p args body p_in (map (v_subst vt) tys) Hmaplen
+  (pred_arg_list pd vt p tys tms (term_rep gamma_valid pd vt pf vv) Hty2) vt vv).
+  (*Simplify LHS*)
+  revert Hty1. unfold sub_body_f.
+  intros.
+  assert (Hall: Forall (fun x : term * vty => term_has_type gamma (fst x) (snd x))
+  (combine (map snd (combine (map (ty_subst_var (s_params p) tys) args) tms))
+     (map snd (map fst (combine (map (ty_subst_var (s_params p) tys) args) tms))))).
+  {
+    inversion Hty2; subst.
+    rewrite map_fst_combine, map_snd_combine; auto;
+    try rewrite !map_length; auto.
+    rewrite map_map. simpl.
+    rewrite <- Hargs in H7.
+    rewrite !map_map in H7.
+    clear -H7 Hargs. revert H7.
+    rewrite !Forall_forall; intros.
+    apply H7.
+    erewrite map_ext_in.
+    apply H.
+    intros. simpl. apply ty_subst_equiv; auto.
+    assert (In (snd a) (s_args p)). {
+      rewrite <-Hargs, in_map_iff. exists a; auto.
+    }
+    pose proof (s_args_wf p).
+    apply check_args_prop with(x:=(snd a)) in H2; auto.
+  }
+  assert (Htysubst: formula_typed gamma (ty_subst_wf_fmla (s_params p) tys body)).
+  {
+    inversion Hty2; subst.
+    apply ty_subst_wf_fmla_typed; auto.
+    apply (NoDup_map_sublist _ _ args); auto.
+    apply fmla_fv_nodup.
+  }
+  rewrite safe_sub_fs_rep with(Hall:=Hall)(Hty2:=Htysubst).
+  2: {
+    rewrite map_fst_combine; try rewrite !map_length; auto.
+    eapply NoDup_map_inv with(f:=fst). rewrite !map_map.
+    simpl. auto.
+  }
+  erewrite ty_subst_wf_fmla_rep; auto.
+  2: apply (NoDup_map_sublist _ _ args); auto;
+    apply fmla_fv_nodup.
+  Unshelve.
+  all: auto.
+  2: apply s_params_Nodup.
+  (*Now we must show that these [term_rep]s are equal*)
+  erewrite fmla_rep_irrel.
+  apply fmla_change_vv.
+  (*Boils down to showing that the upd_vv_args and val_with_args commute*)
+  intros x Hinx.
+  unfold upd_vv_args.
+  assert (In x args). {
+    apply Hfvargs; auto.
+  }
+  destruct (In_nth _ _ vs_d H) as [i [Hi Hx]]; subst.
+  assert (Heq1: nth i (sym_sigma_args p (map (v_subst vt) tys)) s_int =
+  v_subst (vt_with_args vt (s_params p) (map (v_subst vt) tys)) (snd (nth i args vs_d))).
+  {
+    unfold sym_sigma_args, ty_subst_list_s.
+    rewrite <- Hargs, !map_map.
+    rewrite map_nth_inbound with (d2:=vs_d); auto.
+    rewrite <- v_subst_vt_with_args'; auto; [| apply s_params_Nodup].
+    rewrite <- funsym_subst_eq; auto; [| apply s_params_Nodup].
+    f_equal. apply ty_subst_equiv.
+    intros y Hiny.
+    pose proof (s_args_wf p).
+    apply check_args_prop with(x:=(snd (nth i args vs_d))) in H0.
+    - apply H0. auto.
+    - rewrite <- Hargs. rewrite in_map_iff.
+      exists (nth i args vs_d); auto.
+  }
+  erewrite val_with_args_in with(Heq:=Heq1); auto.
+  2: { apply NoDup_map_inv in Hnargs; auto. }
+  2: { unfold sym_sigma_args, ty_subst_list_s. rewrite map_length; auto.
+    rewrite <- Hargs, map_length; auto. }
+  (*Now simplify the other side*)
+  assert (Hnthx: nth i (map fst (combine (map (ty_subst_var (s_params p) tys) args) tms)) vs_d =
+  (ty_subst_var (s_params p) tys (nth i args vs_d))).
+  {
+    rewrite map_fst_combine; try rewrite !map_length; auto.
+    rewrite map_nth_inbound with (d2:=vs_d); auto.
+  }
+  assert (Heq2: nth i
+  (map (v_subst vt)
+     (map snd (map fst (combine (map (ty_subst_var (s_params p) tys) args) tms)))) s_int =
+  v_subst vt (snd (ty_subst_var (s_params p) tys (nth i args vs_d)))).
+  {
+    rewrite map_fst_combine; try rewrite !map_length; auto.
+    unfold ty_subst_var. simpl. rewrite !map_map. simpl.
+    rewrite map_nth_inbound with (d2:=vs_d); auto. 
+  }
+  erewrite val_with_args_in' with(i:=i)(Heq:=Heq2); auto;
+  try rewrite !map_length; auto.
+  (*TODO: put goals together*)
+  2: rewrite map_fst_combine; try rewrite !map_length; auto;
+    apply (NoDup_map_inv fst); rewrite !map_map; simpl; auto.
+  2: rewrite combine_length, map_length; lia.
+  rewrite !dom_cast_compose.
+  (*Now we simplify each of the hnths*)
+  assert (Hi2: i <
+  Datatypes.length (map snd (map fst (combine (map (ty_subst_var (s_params p) tys) args) tms)))).
+  { rewrite !map_length, combine_length, !map_length; lia. }
+  erewrite map_arg_list_nth with(Hi:=Hi2).
+  (*And the other side (harder)*)
+  unfold fun_arg_list.
+  assert (Heq3: v_subst vt (ty_subst (s_params p) tys (nth i (s_args p) vty_int)) =
+  nth i (ty_subst_list_s (s_params p) (map (v_subst vt) tys) (s_args p)) s_int).
+  {
+    unfold ty_subst_list_s.
+    rewrite !map_nth_inbound with (d2:=vty_int); auto.
+    apply funsym_subst_eq; auto.
+    apply s_params_Nodup.
+    rewrite <- Hargs, map_length; auto.
+  }
+  assert (Hty3: term_has_type gamma (nth i tms tm_d) (ty_subst (s_params p) tys (nth i (s_args p) vty_int))). {
+    apply map_arg_list_nth_ty with(i:=i) in Hall; try rewrite !map_length; auto.
+    2: rewrite combine_length, map_length; lia.
+    rewrite map_snd_combine, map_fst_combine in Hall;
+    try rewrite !map_length; auto.
+    rewrite <- Hargs.
+    rewrite !map_map in Hall.
+    rewrite map_nth_inbound with(d2:=vs_d) in Hall; auto.
+    rewrite map_nth_inbound with (d2:=vs_d); auto.
+    unfold ty_subst_var in Hall. simpl in Hall.
+    erewrite ty_subst_equiv; auto.
+    (*TODO: repetitive*)
+    intros y Hiny.
+    pose proof (s_args_wf p).
+    apply check_args_prop with (x:=snd (nth i args vs_d)) in H0; auto.
+    rewrite <- Hargs. rewrite in_map_iff. exists (nth i args vs_d); auto.
+  }
+  erewrite (get_arg_list_hnth pd vt p tys tms (term_rep gamma_valid pd vt pf vv) 
+  (ltac:(intros; apply term_rep_irrel)) (s_params_Nodup p) (proj1' (pred_val_inv Hty2)) (proj1' (proj2' (pred_val_inv Hty2)))
+  (proj2' (proj2' (pred_val_inv Hty2)))).
+  Unshelve.
+  3: exact Heq3.
+  3: exact Hty3.
+  2: rewrite <-Hargs, map_length; auto.
+  rewrite !dom_cast_compose.
+  repeat match goal with
+  | |- context [dom_cast ?d ?H ?x] => generalize dependent H
+  end.
+  repeat match goal with
+  | |- context [term_rep ?g ?pd ?vt ?pf ?vv ?t ?ty ?Hty] =>
+    generalize dependent Hty
+  end.
+  rewrite map_snd_combine; [| rewrite !map_length; auto].
+  rewrite !map_fst_combine; [| rewrite !map_length; auto].
+  generalize dependent (ty_subst (s_params p) tys (nth i (s_args p) vty_int)).
+  generalize dependent (nth i (map snd (map (ty_subst_var (s_params p) tys) args)) vty_int).
+  intros. assert (v = v0). {
+    eapply term_has_type_unique. apply t. auto.
+  }
+  subst. assert (e = e0). apply UIP_dec. apply sort_eq_dec.
+  subst. f_equal. apply term_rep_irrel.
+Qed.
+
+Definition get_rec_pred_body_args (gamma: context) (p: predsym) :
+option (formula * list vsymbol) :=
+fold_right (fun x acc =>
+  match x with
+  | pred_def f1 args t => if predsym_eq_dec p f1 then Some (t, args) else acc 
+  | _ => acc
+  end) None (concat (mutfuns_of_context gamma)).
+
+Lemma get_rec_pred_body_args_some_aux gamma p t args:
+  get_rec_pred_body_args gamma p = Some (t, args) ->
+  In (pred_def p args t) (concat (mutfuns_of_context gamma)).
+Proof.
+  unfold get_rec_pred_body_args.
+  induction (concat (mutfuns_of_context gamma)); simpl; try discriminate.
+  destruct a; auto.
+  destruct (predsym_eq_dec p p0); subst; auto.
+  intros C; inversion C; subst. auto.
+Qed.
+
+Lemma get_rec_pred_body_args_some gamma p t args:
+  get_rec_pred_body_args gamma p = Some (t, args) ->
+  exists fs,
+  In fs (mutfuns_of_context gamma) /\
+  In (pred_def p args t) fs.
+Proof.
+  intros.
+  apply get_rec_pred_body_args_some_aux in H.
+  rewrite in_concat in H.
+  auto.
+Qed.
+
+Definition get_nonrec_pred_body_args gamma p : option (formula * list vsymbol) :=
+  fold_right (fun x acc =>
+    match x with
+    | nonrec_def (pred_def p1 args body) => 
+      if predsym_eq_dec p p1 then Some (body, args)
+      else acc
+    | _ => acc
+    end) None gamma.
+
+Lemma get_nonrec_pred_body_args_some gamma p body args :
+  get_nonrec_pred_body_args gamma p = Some (body, args) ->
+  In (nonrec_def (pred_def p args body)) gamma.
+Proof.
+  induction gamma; simpl; try discriminate.
+  destruct a; auto. destruct f; auto.
+  destruct (predsym_eq_dec p p0); subst; auto.
+  intro C; inversion C; subst. auto.
+Qed.
+
+Definition get_pred_body_args gamma p : option (formula * list vsymbol) :=
+  match (get_rec_pred_body_args gamma p) with
+  | None => get_nonrec_pred_body_args gamma p
+  | x => x
+  end.
+
+Lemma get_pred_body_args_some gamma p body args:
+  get_pred_body_args gamma p = Some (body, args) ->
+  pred_defined gamma p args body.
+Proof.
+  intros. unfold get_pred_body_args in H.
+  unfold pred_defined.
+  destruct (get_rec_pred_body_args gamma p) eqn : Hrec.
+  - inversion H; subst.
+    apply get_rec_pred_body_args_some in Hrec. auto.
+  - apply get_nonrec_pred_body_args_some in H; auto.
+Qed.
+
+Definition unfold_p (gamma: context) (p: predsym) (fmla: formula) :=
+  match (get_pred_body_args gamma p) with
+  | Some (t, args) => unfold_p_aux p fmla args t
+  | None => fmla
+  end.
+
+Definition unfold_p_single (gamma: context) (p: predsym) (i: nat) 
+  (fmla: formula)
+   :=
+  match (get_pred_body_args gamma p) with
+  | Some (t, args) =>
+    let l := find_pred_app_f p fmla in
+    if Nat.ltb i (length l) then
+      unfold_p_single_aux p fmla args t (nth i l (nil, nil))
+    else fmla
+  | _ => fmla
+  end.
+
+Lemma sub_body_f_ty (p: predsym) gamma args body tys tms:
+  Forall (valid_type gamma) tys ->
+  NoDup (map fst (fmla_fv body)) ->
+  Forall (fun x : string * vty * term => term_has_type gamma (snd x) (snd (fst x)))
+  (combine (map (ty_subst_var (s_params p) tys) args) tms) ->
+  formula_typed gamma body ->
+  formula_typed gamma (sub_body_f p args body tys tms).
+Proof.
+  intros.
+  unfold sub_body_f.
+  apply safe_sub_fs_ty.
+  - apply ty_subst_wf_fmla_typed; auto.
+  - auto.
+Qed. 
+
+Lemma sub_pred_body_p_typed gamma p args body tys tms f1:
+  formula_typed gamma (Fpred p tys tms) ->
+  formula_typed gamma (sub_body_f p args body tys tms) ->
+  formula_typed gamma f1 ->
+  formula_typed gamma (sub_pred_body_f p args body tys tms f1).
+Proof.
+  intros. unfold sub_pred_body_f. 
+  apply (proj_fmla (replace_fmla_ty _ _ H H0) f1); auto.
+Qed.
+
+Lemma find_pred_app_tys gamma (p: predsym) x y t f:
+  (forall ty (Hty: term_has_type gamma t ty) 
+    (Hin: In (x, y) (find_pred_app_t p t)),
+    formula_typed gamma (Fpred p x y)) /\
+  (forall (Hty: formula_typed gamma f) 
+    (Hin: In (x, y) (find_pred_app_f p f)),
+    formula_typed gamma (Fpred p x y)).
+Proof.
+  revert t f; apply term_formula_ind; simpl; intros; auto;
+  try contradiction.
+  - cbn in Hin.
+    inversion Hty; subst.
+    rewrite in_concat in Hin.
+    destruct Hin as [l' [Hinl' Hinxy]].
+    rewrite in_map_iff in Hinl'.
+    destruct Hinl' as [tm [Hl' Hintm]]; subst.
+    rewrite Forall_forall in H.
+    destruct (In_nth _ _ tm_d Hintm) as [j [Hj Hx]]; subst.
+    eapply H. apply Hintm. all: auto.
+    rewrite Forall_forall in H10.
+    eapply (H10 (nth j l1 tm_d, (nth j (map (ty_subst (s_params f1) l) (s_args f1)) vty_int))).
+    rewrite in_combine_iff; try rewrite map_length; auto.
+    exists j. split; auto. intros. f_equal; apply nth_indep; try rewrite map_length; auto. lia.
+  - inversion Hty; subst. cbn in Hin.
+    rewrite in_app_iff in Hin. destruct Hin; [apply (H (snd v)) | apply (H0 ty)]; auto.
+  - cbn in Hin. inversion Hty; subst.
+    rewrite !in_app_iff in Hin; destruct_all;
+    [apply H | apply (H0 ty) | apply (H1 ty)]; auto.
+  - cbn in Hin. inversion Hty; subst.
+    rewrite in_app_iff in Hin.
+    destruct Hin.
+    + apply (H v); auto.
+    + rewrite in_concat in H1.
+      destruct H1 as [l' [Hinl' Hinxy]].
+      rewrite in_map_iff in Hinl'.
+      destruct Hinl' as [pt [Hl' Hpt]]; subst.
+      rewrite Forall_map, Forall_forall in H0.
+      apply (H0 pt Hpt ty); auto.
+  - cbn in Hin. inversion Hty; subst. apply H; auto.
+  - cbn in Hin.
+    rewrite in_app_iff in Hin. destruct Hin.
+  + destruct (predsym_eq_dec p0 p); subst; auto; try contradiction.
+    simpl in H0. destruct H0 as [Heq | []]; inversion Heq; subst.
+    auto.
+  + inversion Hty; subst.
+    rewrite in_concat in H0.
+    destruct H0 as [l' [Hinl' Hinxy]].
+    rewrite in_map_iff in Hinl'.
+    destruct Hinl' as [tm [Hl' Hintm]]; subst.
+    rewrite Forall_forall in H.
+    destruct (In_nth _ _ tm_d Hintm) as [j [Hj Hx]]; subst.
+    eapply H. apply Hintm. auto.
+    rewrite Forall_forall in H9.
+    eapply (H9 (nth j tms tm_d, (nth j (map (ty_subst (s_params p0) tys) (s_args p0)) vty_int))).
+    rewrite in_combine_iff; try rewrite map_length; auto.
+    exists j. split; auto. intros. f_equal; apply nth_indep; try rewrite map_length; auto. lia.
+    auto.
+  - cbn in Hin. inversion Hty; subst. apply H; auto.
+  - cbn in Hin. rewrite in_app_iff in Hin. inversion Hty; subst.
+    destruct Hin; [apply (H v) | apply (H0 v)]; auto.
+  - cbn in Hin. rewrite in_app_iff in Hin. inversion Hty; subst.
+    destruct Hin; [apply H | apply H0]; auto.
+  - inversion Hty; subst. cbn in Hin.
+    rewrite in_app_iff in Hin. destruct Hin; 
+    [apply (H (snd v)) | apply H0]; auto.
+  - cbn in Hin. inversion Hty; subst.
+    rewrite !in_app_iff in Hin; destruct_all; auto.
+  - cbn in Hin. inversion Hty; subst.
+    rewrite in_app_iff in Hin.
+    destruct Hin.
+    + apply (H v); auto.
+    + rewrite in_concat in H1.
+      destruct H1 as [l' [Hinl' Hinxy]].
+      rewrite in_map_iff in Hinl'.
+      destruct Hinl' as [pt [Hl' Hpt]]; subst.
+      rewrite Forall_map, Forall_forall in H0.
+      apply (H0 pt Hpt); auto.
+Qed.
+
+Definition find_pred_app_t_ty gamma t ty Hty f1 x y:=
+  (proj_tm (find_pred_app_tys gamma f1 x y) t) ty Hty.
+Definition find_pred_app_f_ty gamma f  Hty f1 x y:=
+  (proj_fmla (find_pred_app_tys gamma f1 x y) f) Hty.
+
+Lemma sub_body_f_ty' gamma (p: predsym)
+(a: list vty * list term)
+(args: list (string * vty))
+(body: formula)
+(Hnargs: NoDup (map fst args))
+(Htyb: formula_typed gamma body)
+(Hfvargs: sublist (fmla_fv body) args)
+(Hargs: map snd args = s_args p)
+(Hall: Forall (valid_type gamma) (fst a))
+(Halen1: Datatypes.length (snd a) = Datatypes.length (s_args p))
+(Hallty: Forall (fun x : term * vty => term_has_type gamma (fst x) (snd x))
+        (combine (snd a) (map (ty_subst (s_params p) (fst a)) (s_args p)))):
+formula_typed gamma (sub_body_f p args body (fst a) (snd a)).
+Proof.
+  apply sub_body_f_ty; auto.
+  + eapply NoDup_map_sublist. apply Hnargs. all: auto.
+    apply fmla_fv_nodup.
+  + rewrite !Forall_forall. intros x.
+    assert (length (snd a) = length args). {
+      rewrite Halen1, <- Hargs, map_length; auto.
+    }
+    rewrite in_combine_iff; try rewrite !map_length; auto.
+    intros [i [Hi Hx]].
+    specialize (Hx vs_d tm_d); subst; simpl.
+    rewrite !map_nth_inbound with (d2:=vs_d); auto.
+    simpl.
+    revert Hallty. rewrite !Forall_forall. intros.
+    apply specialize_combine with(d1:=tm_d)(d2:=vty_int)(i:=i) in Hallty;
+    auto; try rewrite !map_length; auto.
+    2: rewrite H; auto. (*why doesn't lia work?*)
+    simpl in Hallty.
+    rewrite map_nth_inbound with (d2:=vty_int) in Hallty;
+    [| rewrite <- Halen1, H; auto].
+    rewrite <- Hargs in Hallty.
+    rewrite map_nth_inbound with (d2:=vs_d) in Hallty; auto.
+    rewrite <- ty_subst_equiv; auto.
+    pose proof (s_args_wf p).
+    apply check_args_prop with (x:=snd (nth i args vs_d)) in H0;
+    auto. rewrite <- Hargs. rewrite in_map_iff.
+    exists (nth i args vs_d). split; auto. apply nth_In; auto.
+Qed.
+
+(*Lemma sub_pred_body_f_ty gamma (p: predsym)
+(a: list vty * list term)
+(args: list (string * vty))
+(body: term)
+(Hnargs: NoDup (map fst args))
+(Htyb: term_has_type gamma body)
+(Hfvargs: sublist (tm_fv body) args)
+(Hargs: map snd args = s_args f)
+(base: formula)
+(Htya: term_has_type gamma (Tfun f (fst a) (snd a)) (ty_subst (s_params f) (fst a) (f_ret f)))
+(H: formula_typed gamma base)
+(Hall: Forall (valid_type gamma) (fst a))
+(Halen1: Datatypes.length (snd a) = Datatypes.length (s_args f))
+(Hallty: Forall (fun x : term * vty => term_has_type gamma (fst x) (snd x))
+        (combine (snd a) (map (ty_subst (s_params f) (fst a)) (s_args f))))
+(Hsub: sublist (type_vars (f_ret f)) (s_params f)):
+formula_typed gamma (sub_fun_body_f f args body (fst a) (snd a) base).
+Proof.
+  eapply sub_fun_body_f_typed. apply Htya. all: auto. 
+  rewrite ty_subst_equiv; auto.
+  apply sub_body_t_ty'; auto.
+Qed.*)
+(*
+(*Typing for [unfold_p]*)
+*)
+Lemma unfold_p_ty_aux {gamma} (gamma_valid: valid_context gamma)
+(p: predsym) l base args body
+(Hnargs : NoDup (map fst args))
+(Htyb: formula_typed gamma body)
+(Hfvargs: sublist (fmla_fv body) args)
+(Hargs: map snd args = s_args p)
+(Hl: forall x y, In (x, y) l -> 
+  formula_typed gamma (Fpred p x y)):
+formula_typed gamma base ->
+formula_typed gamma
+  (fold_left (fun acc x => sub_pred_body_f p args body (fst x) (snd x) acc) l base).
+Proof.
+  revert Hl.
+  generalize dependent base.
+  induction l; simpl; intros; auto.
+  apply IHl; auto.
+  specialize (Hl (fst a) (snd a) ltac:(destruct a; auto)).
+  apply sub_pred_body_p_typed; auto.
+  inversion Hl; subst.
+  apply sub_body_f_ty'; auto.
+Qed.
+
+Lemma unfold_p_ty {gamma} (gamma_valid: valid_context gamma)
+  (p: predsym) (fmla: formula)
+  (Hty1: formula_typed gamma fmla):
+  formula_typed gamma (unfold_p gamma p fmla).
+Proof.
+  unfold unfold_p.
+  destruct (get_pred_body_args gamma p) eqn : Hfunbody; auto.
+  destruct p0 as [body args].
+  (*Typing info*)
+  apply get_pred_body_args_some in Hfunbody.
+  pose proof (pred_defined_valid gamma_valid Hfunbody) as Hdef.
+  simpl in Hdef.
+  destruct Hdef as [Htyb [Hfvargs [Hsubvars [Hnargs Hargs]]]].
+  apply unfold_p_ty_aux; auto.
+  intros. eapply find_pred_app_f_ty. 2: apply H. auto.
+Qed.
+
+(*And now we prove the correctness*)
+Lemma unfold_p_rep {gamma} (gamma_valid: valid_context gamma) 
+  (p: predsym) (fmla: formula)
+  (pd: pi_dom) (pf: pi_funpred gamma_valid pd)
+  (pf_full: full_interp gamma_valid pd pf)
+  (vt: val_typevar) (vv: val_vars pd vt)
+  (Hty1: formula_typed gamma fmla)
+  (Hty2: formula_typed gamma (unfold_p gamma p fmla)):
+  formula_rep gamma_valid pd vt pf vv (unfold_p gamma p fmla) Hty2 =
+  formula_rep gamma_valid pd vt pf vv fmla Hty1.
+Proof.
+  revert Hty2.
+  unfold unfold_p.
+  destruct (get_pred_body_args gamma p) eqn : Hfunbody;
+  [|intros; apply fmla_rep_irrel].
+  destruct p0 as [body args]. intros.
+  (*Typing info*)
+  apply get_pred_body_args_some in Hfunbody.
+  pose proof (pred_defined_valid gamma_valid Hfunbody) as Hdef.
+  simpl in Hdef.
+  destruct Hdef as [Htyb [Hfvargs [Hsubvars [Hnargs Hargs]]]].
+  revert Hty2. unfold unfold_p_aux.
+  (*Because fold_left, we ned to generalize base*)
+  assert (forall l base Hty2 Hty3
+    (Hl: forall x y, In (x, y) l ->
+      formula_typed gamma (Fpred p x y)),
+    formula_rep gamma_valid pd vt pf vv base Hty2 =
+    formula_rep gamma_valid pd vt pf vv fmla Hty1 ->
+    formula_rep gamma_valid pd vt pf vv
+      (fold_left (fun acc x => sub_pred_body_f p args body (fst x) (snd x) acc) l base)
+    Hty3 =
+    formula_rep gamma_valid pd vt pf vv fmla Hty1).
+  {
+    induction l; simpl; intros.
+    - erewrite fmla_rep_irrel. rewrite H. apply fmla_rep_irrel.
+    - assert (Htya: formula_typed gamma (Fpred p (fst a) (snd a))).
+        { apply Hl. left; destruct a; auto. }
+      (*Hardest part: proving typing*)
+      (*assert (Hsub: sublist (type_vars (f_ret )) (s_params f)). {
+        pose proof (f_ret_wf f).
+        apply check_sublist_prop in H0; auto.
+      }*)
+      assert (Hty4: formula_typed gamma (sub_body_f p args body (fst a) (snd a))). {
+        inversion Htya; subst.
+        apply sub_body_f_ty'; auto.
+      }
+      assert (Hty5: formula_typed gamma (sub_pred_body_f p args body (fst a) (snd a) base)).
+      {
+        inversion Htya; subst; auto.
+        apply sub_pred_body_p_typed; auto.
+      }
+      apply IHl with (Hty2:=Hty5).
+      { intros; apply Hl; auto. }
+      revert Hty4.
+      unfold sub_pred_body_f.
+      intros.
+      erewrite replace_fmla_f_rep.
+      apply H. apply Htya. apply Hty4.
+      intros.
+      erewrite sub_body_f_rep. reflexivity. all: auto.
+      + inversion Hty0; subst. 
+        rewrite H6. rewrite <- Hargs, !map_length; auto.
+      + inversion Hty0; subst. auto.
+  }
+  intros.
+  eapply H. 2: reflexivity.
+  (*Need that [find_fun_app_f] well_typed*)
+  intros. eapply find_pred_app_f_ty. 2: apply H0. auto.
+Qed.
+
+(*And the results for [unfold_f_single]*)
+Lemma unfold_p_single_rep {gamma} (gamma_valid: valid_context gamma) 
+  (p: predsym) (fmla: formula)
+  (pd: pi_dom) (pf: pi_funpred gamma_valid pd)
+  (pf_full: full_interp gamma_valid pd pf)
+  (vt: val_typevar) (vv: val_vars pd vt)
+  (i: nat)
+  (Hty1: formula_typed gamma fmla)
+  (Hty2: formula_typed gamma (unfold_p_single gamma p i fmla)):
+  formula_rep gamma_valid pd vt pf vv (unfold_p_single gamma p i fmla) Hty2 =
+  formula_rep gamma_valid pd vt pf vv fmla Hty1.
+Proof.
+  revert Hty2.
+  unfold unfold_p_single.
+  destruct (get_pred_body_args gamma p) eqn : Hfunbody;
+  [|intros; apply fmla_rep_irrel].
+  destruct p0 as [body args].
+  destruct (Nat.ltb_spec0 i (length (find_pred_app_f p fmla)));
+  [|intros; apply fmla_rep_irrel].
+  intros.
+  apply get_pred_body_args_some in Hfunbody.
+  pose proof (pred_defined_valid gamma_valid Hfunbody) as Hdef.
+  simpl in Hdef.
+  destruct Hdef as [Htyb [Hfvargs [Hsubvars [Hnargs Hargs]]]].
+  unfold unfold_p_single_aux, sub_pred_body_f.
+  set (vs := (fst (nth i (find_pred_app_f p fmla) ([], [])))).
+  set (ts := (snd (nth i (find_pred_app_f p fmla) ([], [])))).
+  pose proof (find_pred_app_f_ty gamma fmla Hty1 p vs ts) as Htyi.
+  prove_hyp Htyi.
+  {
+    assert ((vs, ts) = nth i (find_pred_app_f p fmla) (nil,nil)). {
+      unfold vs, ts.
+      destruct (nth i (find_pred_app_f p fmla) (nil,nil)); auto.
+    }
+    rewrite H. apply nth_In; auto.
+  }
+   (*Hardest part: proving typing*)
+   (*assert (Hsub: sublist (type_vars (f_ret f)) (s_params f)). {
+    pose proof (f_ret_wf f).
+    apply check_sublist_prop in H; auto.
+  }*)
+  assert (Hty4: formula_typed gamma (sub_body_f p args body vs ts)). {
+    inversion Htyi; subst.
+    apply sub_body_f_ty'; auto.
+  }
+  erewrite replace_fmla_f_rep.
+  reflexivity. apply Htyi.
+  apply Hty4.
+  intros.
+  erewrite sub_body_f_rep. reflexivity. all: auto.
+  + inversion Hty0; subst. 
+    rewrite H5. rewrite <- Hargs, !map_length; auto.
+  + inversion Hty0; subst. auto.
+Qed.
+
+(*And typing*)
+
+Lemma unfold_p_single_ty {gamma} (gamma_valid: valid_context gamma)
+  (p: predsym) (fmla: formula)
+  (Hty1: formula_typed gamma fmla) (i: nat):
+  formula_typed gamma (unfold_p_single gamma p i fmla).
+Proof.
+  unfold unfold_p_single.
+  destruct (get_pred_body_args gamma p) eqn : Hfunbody; auto.
+  destruct p0 as [body args].
+  destruct (Nat.ltb_spec0 i (length (find_pred_app_f p fmla))); auto.
+  (*Typing info*)
+  apply get_pred_body_args_some in Hfunbody.
+  pose proof (pred_defined_valid gamma_valid Hfunbody) as Hdef.
+  simpl in Hdef.
+  destruct Hdef as [Htyb [Hfvargs [Hsubvars [Hnargs Hargs]]]].
+  unfold unfold_f_single_aux.
+  set (vs := (fst (nth i (find_pred_app_f p fmla) ([], [])))).
+  set (ts := (snd (nth i (find_pred_app_f p fmla) ([], [])))).
+  pose proof (find_pred_app_f_ty gamma fmla Hty1 p vs ts) as Htyi.
+  prove_hyp Htyi.
+  {
+    assert ((vs, ts) = nth i (find_pred_app_f p fmla) (nil,nil)). {
+      unfold vs, ts.
+      destruct (nth i (find_pred_app_f p fmla) (nil,nil)); auto.
+    }
+    rewrite H. apply nth_In; auto.
+  }
+  inversion Htyi; subst.
+  apply sub_pred_body_p_typed; auto.
+  apply sub_body_f_ty'; auto.
+Qed.
