proofs/proofsystem/Rewrite.v
@@ -1,0 +1,515 @@
+(*Replace terms and formulas with equivalent ones*)
+Require Import Typechecker.
+Require Export Denotational.
+Set Bullet Behavior "Strict Subproofs".
+
+(*Substitute a term for a term in a term or formula*)
+Section ReplaceTm.
+
+Variable tm_o tm_n: term.
+
+Fixpoint replace_tm_t (t: term) :=
+  if term_eq_dec tm_o t then tm_n else
+  (*Just a bunch of recursive cases*)
+  match t with
+  | Tfun f tys tms => Tfun f tys (map replace_tm_t tms)
+  | Tlet t1 v t2 =>
+    Tlet (replace_tm_t t1) v 
+    (*Avoid capture -*)
+    (if in_bool vsymbol_eq_dec v (tm_fv tm_o) then t2
+    else (replace_tm_t t2))
+  | Tif f t1 t2 =>
+    Tif (replace_tm_f f) (replace_tm_t t1) (replace_tm_t t2)
+  | Tmatch tm ty ps =>
+    Tmatch (replace_tm_t tm) ty
+    (map (fun x => (fst x, 
+      if existsb (fun v => in_bool vsymbol_eq_dec v (tm_fv tm_o))
+       (pat_fv (fst x))
+         then
+      snd x else (replace_tm_t (snd x)))) ps)
+  | Teps f v =>
+    Teps (if in_bool vsymbol_eq_dec v (tm_fv tm_o) then f else
+      replace_tm_f f) v
+  | _ => t
+  end
+with replace_tm_f (f: formula) :=
+  match f with
+  | Fpred p tys tms =>
+    Fpred p tys (map replace_tm_t tms)
+  | Fquant q v f =>
+    Fquant q v (if in_bool vsymbol_eq_dec v (tm_fv tm_o) then f else
+      replace_tm_f f)
+  | Feq ty t1 t2 => Feq ty (replace_tm_t t1) (replace_tm_t t2)
+  | Fbinop b f1 f2 => Fbinop b (replace_tm_f f1) (replace_tm_f f2)
+  | Fnot f => Fnot (replace_tm_f f)
+  | Flet t v f => Flet (replace_tm_t t) v
+    (if in_bool vsymbol_eq_dec v (tm_fv tm_o) then f 
+      else (replace_tm_f f))
+  | Fif f1 f2 f3 => Fif (replace_tm_f f1) (replace_tm_f f2)
+    (replace_tm_f f3)
+  | Fmatch tm ty ps =>
+    Fmatch (replace_tm_t tm) ty
+    (map (fun x => (fst x, 
+      if existsb (fun v => in_bool vsymbol_eq_dec v (tm_fv tm_o))
+      (pat_fv (fst x))
+        then
+      snd x else (replace_tm_f (snd x)))) ps)
+  | _ => f
+  end.
+
+End ReplaceTm.
+
+(*Typing lemma*)
+
+
+Ltac tm_eq t1 t2 := destruct (term_eq_dec t1 t2).
+
+Ltac simpl_tys :=
+  subst; auto;
+  match goal with
+  | H: term_has_type ?g ?t ?v1, H2: term_has_type ?g ?t ?v2 |- _ =>
+    let Heq := fresh "Heq" in
+    assert (Heq: v1 = v2) by (apply (term_has_type_unique _ _ _ _ H H2));
+    subst; auto
+  end.
+
+Ltac destruct_if :=
+  match goal with
+  | |- context [if ?b then ?c else ?d] =>
+    destruct b
+  end.
+
+Ltac tm_case :=
+  match goal with
+  | |- context [term_eq_dec ?t1 ?t2] =>
+    destruct (term_eq_dec t1 t2)
+  end.
+
+Lemma replace_tm_ty {gamma: context} tm_o tm_n
+  ty1 (Hty1: term_has_type gamma tm_o ty1)
+  (Hty2: term_has_type gamma tm_n ty1) t f:
+  (forall (ty2: vty) (Hty: term_has_type gamma t ty2),
+    term_has_type gamma (replace_tm_t tm_o tm_n t) ty2
+  ) /\
+  (forall (Hty: formula_typed gamma f),
+    formula_typed gamma (replace_tm_f tm_o tm_n f)).
+Proof.
+  revert t f. apply term_formula_ind; intros; cbn;
+  try tm_case; try simpl_tys; inversion Hty; subst;
+  try case_in; constructor; auto;
+  (*solve some easy ones*)
+  try solve[rewrite map_length; auto];
+  try solve[rewrite null_map; auto];
+  (*Deal with pattern match cases*)
+  try(intros x Hx; rewrite in_map_iff in Hx;
+    destruct Hx as [t [Hx Hint]]; subst; simpl; auto;
+    destruct (existsb _ _); auto; 
+    rewrite Forall_map, Forall_forall in H0; auto).
+  (*Only function and pred cases left - these are the same
+    but annoying*)
+  - revert H10 H. rewrite !Forall_forall; intros.
+    (*Annoying because of combine*)
+    rewrite in_combine_iff in H0 by (rewrite !map_length; auto).
+    destruct H0 as [i [Hi Hx]].
+    specialize (Hx tm_d vty_int). subst. simpl.
+    rewrite map_length in Hi.
+    rewrite map_nth_inbound with (d2:=tm_d); auto.
+    apply H. apply nth_In. auto.
+    specialize (H10 ((nth i l1 tm_d), (nth i (map (ty_subst (s_params f1) l) (s_args f1)) vty_int))).
+    apply H10.
+    rewrite in_combine_iff by (rewrite map_length; auto).
+    exists i. split; auto. intros.
+    f_equal; apply nth_indep; rewrite ?map_length; lia.
+  - revert H8 H. rewrite !Forall_forall; intros.
+    (*Annoying because of combine*)
+    rewrite in_combine_iff in H0 by (rewrite !map_length; auto).
+    destruct H0 as [i [Hi Hx]].
+    specialize (Hx tm_d vty_int). subst. simpl.
+    rewrite map_length in Hi.
+    rewrite map_nth_inbound with (d2:=tm_d); auto.
+    apply H. apply nth_In. auto.
+    specialize (H8 ((nth i tms tm_d), (nth i (map (ty_subst (s_params p) tys) (s_args p)) vty_int))).
+    apply H8.
+    rewrite in_combine_iff by (rewrite map_length; auto).
+    exists i. split; auto. intros.
+    f_equal; apply nth_indep; rewrite ?map_length; lia.
+Qed.
+
+(*And now we reason about the semantics:
+  if the term_reps of these two terms are equal, 
+  then substituting in one for the other does not
+  change the semantics*)
+Lemma replace_tm_rep {gamma: context} 
+  (gamma_valid: valid_context gamma)
+  (tm_o tm_n: term) (ty1: vty)
+  (Hty1: term_has_type gamma tm_o ty1)
+  (Hty2: term_has_type gamma tm_n ty1)
+  (pd: pi_dom) (pf: pi_funpred gamma_valid pd)
+  (vt: val_typevar)
+  (*Need to be the same for all vals, not under a
+    particular one*)
+  (Hrep: forall (vv: val_vars pd vt) Hty1 Hty2,
+    term_rep gamma_valid pd vt pf vv tm_o ty1 Hty1 =
+    term_rep gamma_valid pd vt pf vv tm_n ty1 Hty2)
+  (t: term) (f: formula) :
+  (forall (vv: val_vars pd vt) (ty2: vty)
+    (Htyt: term_has_type gamma t ty2)
+    (Htysub: term_has_type gamma (replace_tm_t tm_o tm_n t) ty2),
+    term_rep gamma_valid pd vt pf vv (replace_tm_t tm_o tm_n t) ty2 Htysub =
+    term_rep gamma_valid pd vt pf vv t ty2 Htyt
+  ) /\
+  (forall (vv: val_vars pd vt) 
+    (Hvalf: formula_typed gamma f)
+    (Hvalsub: formula_typed gamma (replace_tm_f tm_o tm_n f)),
+    formula_rep gamma_valid pd vt pf vv (replace_tm_f tm_o tm_n f) Hvalsub =
+    formula_rep gamma_valid pd vt pf vv f Hvalf).
+Proof.
+  revert t f; apply term_formula_ind; simpl; intros;
+  try revert Htysub; try revert Hvalsub; cbn;
+  try tm_case; subst; auto; intros;
+  try simpl_tys; try apply term_rep_irrel.
+  - simpl_rep_full. f_equal. apply UIP_dec. apply vty_eq_dec.
+    f_equal. apply UIP_dec. apply sort_eq_dec.
+    f_equal. apply get_arg_list_ext; rewrite map_length; auto.
+    intros.
+    revert Hty0.
+    rewrite map_nth_inbound with (d2:=tm_d); auto; intros.
+    rewrite Forall_forall in H. apply H. apply nth_In; auto.
+  - simpl_rep_full. (*Tlet*) case_in.
+    + erewrite H. apply term_rep_irrel.
+    + erewrite H. apply H0. (*Um, why don't we need 
+      to know about capture? - aha, because we assert
+      (through the Hrep assumption) that these terms are closed,
+      or at least that the val is irrelevant. So we really could
+      substitute under binders*)
+  - (*Tif*)
+    simpl_rep_full. erewrite H, H0, H1. reflexivity.
+  - (*Tmatch*)
+    simpl_rep_full.
+    iter_match_gen Htysub Htmsub Hpatsub Htysub.
+    iter_match_gen Htyt Htmt Hpatt Htyt.
+    clear n. induction ps; simpl; intros; try reflexivity.
+    destruct a as[p1 t1]; simpl in *.
+    rewrite H with (Htyt:=Htyt) at 1.
+    rewrite match_val_single_irrel with(Hval2:=Forall_inv Hpatt).
+    simpl.
+    inversion H0; subst. inversion Htmt; subst.
+    inversion Hpatt; subst.
+    destruct (match_val_single gamma_valid pd vt v p1 (Forall_inv Hpatt)
+    (term_rep gamma_valid pd vt pf vv tm v Htyt)) eqn : Hmatch; auto.
+    destruct (existsb _ _); auto.
+    apply term_rep_irrel.
+  - (*Teps*)
+    simpl_rep_full. f_equal.
+    apply functional_extensionality_dep; intros.
+    replace (f_equal (v_subst vt) (proj2' (ty_eps_inv Htysub))) with
+      (f_equal (v_subst vt) (proj2' (ty_eps_inv Htyt))) by
+      (apply UIP_dec; apply sort_eq_dec).
+    case_in. 
+    + erewrite fmla_rep_irrel. reflexivity.
+    + erewrite H. reflexivity. 
+  - (*Fpred*)
+    simpl_rep_full. f_equal. 
+    apply get_arg_list_ext; rewrite map_length; auto.
+    intros.
+    revert Hty0.
+    rewrite map_nth_inbound with (d2:=tm_d); auto; intros.
+    rewrite Forall_forall in H. apply H. apply nth_In; auto.
+  - (*Fquant*)
+    destruct q; apply all_dec_eq; case_in;
+    split; try (intros [d Hall]; exists d); try (intros Hall d;
+      specialize (Hall d));
+    try solve[erewrite fmla_rep_irrel; apply Hall];
+    erewrite H + erewrite <- H; try apply Hall.
+  - (*Feq*) erewrite H, H0; reflexivity.
+  - (*Fbinop*) erewrite H, H0; reflexivity.
+  - (*Fnot*) erewrite H; reflexivity.
+  - (*Flet*) case_in.
+    + erewrite H. apply fmla_rep_irrel.
+    + erewrite H. apply H0.
+  - (*Fif*) erewrite H, H0, H1; reflexivity.
+  - (*Fmatch*)  
+    iter_match_gen Hvalsub Htmsub Hpatsub Hvalsub.
+    iter_match_gen Hvalf Htmf Hpatf Hvalf.
+    induction ps; simpl; intros; try reflexivity.
+    destruct a as[p1 t1]; simpl in *.
+    rewrite H with (Htyt:=Hvalf) at 1.
+    rewrite match_val_single_irrel with(Hval2:=Forall_inv Hpatf).
+    simpl.
+    inversion H0; subst. inversion Htmf; subst.
+    inversion Hpatf; subst. simpl. simpl_rep_full.
+    (*What is going on here?*)
+    match goal with
+    | |- match ?p1 with | Some l1 => _ | None => _ end =
+      match ?p2 with | Some l2 => _ | None => _ end =>
+      replace p2 with p1 by reflexivity
+    end.
+    destruct (match_val_single gamma_valid pd vt v p1 (Forall_inv Hpatf)
+    (term_rep gamma_valid pd vt pf vv tm v Hvalf)) eqn : Hmatch; auto.
+    destruct (existsb _ _); auto.
+    apply fmla_rep_irrel.
+Qed.
+
+Definition replace_tm_f_rep {gamma: context} 
+(gamma_valid: valid_context gamma)
+(tm_o tm_n: term) (ty1: vty)
+(Hty1: term_has_type gamma tm_o ty1)
+(Hty2: term_has_type gamma tm_n ty1)
+(pd: pi_dom) (pf: pi_funpred gamma_valid pd)
+(vt: val_typevar)
+(Hrep: forall (vv: val_vars pd vt) Hty1 Hty2,
+    term_rep gamma_valid pd vt pf vv tm_o ty1 Hty1 =
+    term_rep gamma_valid pd vt pf vv tm_n ty1 Hty2)
+(f: formula) :=
+proj_fmla (replace_tm_rep gamma_valid tm_o tm_n ty1 Hty1 Hty2
+  pd pf vt Hrep) f.
+
+(*And the same for rewriting/replacing formulas -
+  can we reduce duplication?*)
+
+Section ReplaceFmla.
+
+Variable fmla_o fmla_n: formula.
+
+Fixpoint replace_fmla_t (t: term) :=
+  (*Just a bunch of recursive cases*)
+  match t with
+  | Tfun f tys tms => Tfun f tys (map replace_fmla_t tms)
+  | Tlet t1 v t2 =>
+    Tlet (replace_fmla_t t1) v 
+    (*Avoid capture -*)
+    (if in_bool vsymbol_eq_dec v (fmla_fv fmla_o) then t2
+    else (replace_fmla_t t2))
+  | Tif f t1 t2 =>
+    Tif (replace_fmla_f f) (replace_fmla_t t1) (replace_fmla_t t2)
+  | Tmatch tm ty ps =>
+    Tmatch (replace_fmla_t tm) ty
+    (map (fun x => (fst x, 
+      if existsb (fun v => in_bool vsymbol_eq_dec v (fmla_fv fmla_o))
+       (pat_fv (fst x))
+         then
+      snd x else (replace_fmla_t (snd x)))) ps)
+  | Teps f v =>
+    Teps (if in_bool vsymbol_eq_dec v (fmla_fv fmla_o) then f else
+    replace_fmla_f f) v
+  | _ => t
+  end
+with replace_fmla_f (f: formula) :=
+if formula_eq_dec fmla_o f then fmla_n else
+  match f with
+  | Fpred p tys tms =>
+    Fpred p tys (map replace_fmla_t tms)
+  | Fquant q v f =>
+    Fquant q v (if in_bool vsymbol_eq_dec v (fmla_fv fmla_o) then f else
+    replace_fmla_f f)
+  | Feq ty t1 t2 => Feq ty (replace_fmla_t t1) (replace_fmla_t t2)
+  | Fbinop b f1 f2 => Fbinop b (replace_fmla_f f1) (replace_fmla_f f2)
+  | Fnot f => Fnot (replace_fmla_f f)
+  | Flet t v f => Flet (replace_fmla_t t) v
+    (if in_bool vsymbol_eq_dec v (fmla_fv fmla_o) then f 
+      else (replace_fmla_f f))
+  | Fif f1 f2 f3 => Fif (replace_fmla_f f1) (replace_fmla_f f2)
+    (replace_fmla_f f3)
+  | Fmatch tm ty ps =>
+    Fmatch (replace_fmla_t tm) ty
+    (map (fun x => (fst x, 
+      if existsb (fun v => in_bool vsymbol_eq_dec v (fmla_fv fmla_o))
+      (pat_fv (fst x))
+        then
+      snd x else (replace_fmla_f (snd x)))) ps)
+  | _ => f
+  end.
+
+End ReplaceFmla.
+
+(*Typing lemma*)
+
+Ltac fmla_eq t1 t2 := destruct (formula_eq_dec t1 t2).
+
+Ltac fmla_case :=
+  match goal with
+  | |- context [formula_eq_dec ?t1 ?t2] =>
+    destruct (formula_eq_dec t1 t2)
+  end.
+
+Lemma replace_fmla_ty {gamma: context} fmla_o fmla_n
+  (Hty1: formula_typed gamma fmla_o)
+  (Hty2: formula_typed gamma fmla_n) t f:
+  (forall (ty2: vty) (Hty: term_has_type gamma t ty2),
+    term_has_type gamma (replace_fmla_t fmla_o fmla_n t) ty2
+  ) /\
+  (forall (Hty: formula_typed gamma f),
+    formula_typed gamma (replace_fmla_f fmla_o fmla_n f)).
+Proof.
+  revert t f. apply term_formula_ind; intros; cbn;
+  try fmla_case; try simpl_tys; inversion Hty; subst;
+  try case_in; constructor; auto;
+  (*solve some easy ones*)
+  try solve[rewrite map_length; auto];
+  try solve[rewrite null_map; auto];
+  (*Deal with pattern match cases*)
+  try(intros x Hx; rewrite in_map_iff in Hx;
+    destruct Hx as [t [Hx Hint]]; subst; simpl; auto;
+    destruct (existsb _ _); auto; 
+    rewrite Forall_map, Forall_forall in H0; auto).
+  (*Only function and pred cases left - these are the same
+    but annoying*)
+  - revert H10 H. rewrite !Forall_forall; intros.
+    (*Annoying because of combine*)
+    rewrite in_combine_iff in H0 by (rewrite !map_length; auto).
+    destruct H0 as [i [Hi Hx]].
+    specialize (Hx tm_d vty_int). subst. simpl.
+    rewrite map_length in Hi.
+    rewrite map_nth_inbound with (d2:=tm_d); auto.
+    apply H. apply nth_In. auto.
+    specialize (H10 ((nth i l1 tm_d), (nth i (map (ty_subst (s_params f1) l) (s_args f1)) vty_int))).
+    apply H10.
+    rewrite in_combine_iff by (rewrite map_length; auto).
+    exists i. split; auto. intros.
+    f_equal; apply nth_indep; rewrite ?map_length; lia.
+  - revert H8 H. rewrite !Forall_forall; intros.
+    (*Annoying because of combine*)
+    rewrite in_combine_iff in H0 by (rewrite !map_length; auto).
+    destruct H0 as [i [Hi Hx]].
+    specialize (Hx tm_d vty_int). subst. simpl.
+    rewrite map_length in Hi.
+    rewrite map_nth_inbound with (d2:=tm_d); auto.
+    apply H. apply nth_In. auto.
+    specialize (H8 ((nth i tms tm_d), (nth i (map (ty_subst (s_params p) tys) (s_args p)) vty_int))).
+    apply H8.
+    rewrite in_combine_iff by (rewrite map_length; auto).
+    exists i. split; auto. intros.
+    f_equal; apply nth_indep; rewrite ?map_length; lia.
+Qed.
+
+(*And now we reason about the semantics:
+  if the formula_reps of these two terms are equal, 
+  then substituting in one for the other does not
+  change the semantics*)
+Lemma replace_fmla_rep {gamma: context} 
+  (gamma_valid: valid_context gamma)
+  (fmla_o fmla_n: formula)
+  (Hty1: formula_typed gamma fmla_o)
+  (Hty2: formula_typed gamma fmla_n)
+  (pd: pi_dom) (pf: pi_funpred gamma_valid pd)
+  (vt: val_typevar)
+  (*Need to be the same for all vals, not under a
+    particular one*)
+  (Hrep: forall (vv: val_vars pd vt) Hty1 Hty2,
+    formula_rep gamma_valid pd vt pf vv fmla_o Hty1 =
+    formula_rep gamma_valid pd vt pf vv fmla_n Hty2)
+  (t: term) (f: formula) :
+  (forall (vv: val_vars pd vt) (ty2: vty)
+    (Htyt: term_has_type gamma t ty2)
+    (Htysub: term_has_type gamma (replace_fmla_t fmla_o fmla_n t) ty2),
+    term_rep gamma_valid pd vt pf vv (replace_fmla_t fmla_o fmla_n t) ty2 Htysub =
+    term_rep gamma_valid pd vt pf vv t ty2 Htyt
+  ) /\
+  (forall (vv: val_vars pd vt) 
+    (Hvalf: formula_typed gamma f)
+    (Hvalsub: formula_typed gamma (replace_fmla_f fmla_o fmla_n f)),
+    formula_rep gamma_valid pd vt pf vv (replace_fmla_f fmla_o fmla_n f) Hvalsub =
+    formula_rep gamma_valid pd vt pf vv f Hvalf).
+Proof.
+  revert t f; apply term_formula_ind; simpl; intros;
+  try revert Htysub; try revert Hvalsub; unfold replace_fmla_t,
+  replace_fmla_f; fold replace_fmla_t; fold replace_fmla_f; simpl;
+  try tm_case; subst; auto; intros;
+  try (fmla_case; subst; [erewrite <-Hrep; reflexivity |]);
+  try simpl_tys; try apply term_rep_irrel.
+  - simpl_rep_full. f_equal. apply UIP_dec. apply vty_eq_dec.
+    f_equal. apply UIP_dec. apply sort_eq_dec.
+    f_equal. apply get_arg_list_ext; rewrite map_length; auto.
+    intros.
+    revert Hty0.
+    rewrite map_nth_inbound with (d2:=tm_d); auto; intros.
+    rewrite Forall_forall in H. apply H. apply nth_In; auto.
+  - simpl_rep_full. (*Tlet*) case_in.
+    + erewrite H. apply term_rep_irrel.
+    + erewrite H. apply H0. (*Um, why don't we need 
+      to know about capture? - aha, because we assert
+      (through the Hrep assumption) that these terms are closed,
+      or at least that the val is irrelevant. So we really could
+      substitute under binders*)
+  - (*Tif*)
+    simpl_rep_full. erewrite H, H0, H1. reflexivity.
+  - (*Tmatch*)
+    simpl_rep_full.
+    iter_match_gen Htysub Htmsub Hpatsub Htysub.
+    iter_match_gen Htyt Htmf Hpatf Htyt.
+    induction ps; simpl; intros; try reflexivity.
+    destruct a as[p1 t1]; simpl in *.
+    rewrite H with (Htyt:=Htyt) at 1.
+    rewrite match_val_single_irrel with(Hval2:=Forall_inv Hpatf).
+    simpl.
+    inversion H0; subst. inversion Htmf; subst.
+    inversion Hpatf; subst. simpl. simpl_rep_full.
+    (*What is going on here?*)
+    match goal with
+    | |- match ?p1 with | Some l1 => _ | None => _ end =
+      match ?p2 with | Some l2 => _ | None => _ end =>
+      replace p2 with p1 by reflexivity
+    end.
+    destruct (match_val_single gamma_valid pd vt v p1 (Forall_inv Hpatf)
+    (term_rep gamma_valid pd vt pf vv tm v Htyt)) eqn : Hmatch; auto.
+    destruct (existsb _ _); auto.
+    apply term_rep_irrel.
+  - (*Teps*)
+    simpl_rep_full. f_equal.
+    apply functional_extensionality_dep; intros.
+    replace (f_equal (v_subst vt) (proj2' (ty_eps_inv Htysub))) with
+      (f_equal (v_subst vt) (proj2' (ty_eps_inv Htyt))) by
+      (apply UIP_dec; apply sort_eq_dec).
+    case_in. 
+    + erewrite fmla_rep_irrel. reflexivity.
+    + erewrite H. reflexivity. 
+  - (*Fpred*)
+    simpl_rep_full. f_equal. 
+    apply get_arg_list_ext; rewrite map_length; auto.
+    intros.
+    revert Hty0.
+    rewrite map_nth_inbound with (d2:=tm_d); auto; intros.
+    rewrite Forall_forall in H. apply H. apply nth_In; auto.
+  - (*Fquant*)
+    destruct q; simpl_rep_full; apply all_dec_eq; case_in;
+    split; try (intros [d Hall]; exists d); try (intros Hall d;
+      specialize (Hall d));
+    try solve[erewrite fmla_rep_irrel; apply Hall];
+    erewrite H + erewrite <- H; try apply Hall.
+  - (*Feq*) simpl_rep_full. erewrite H, H0; reflexivity.
+  - (*Fbinop*) simpl_rep_full. erewrite H, H0; reflexivity.
+  - (*Fnot*) simpl_rep_full. erewrite H; reflexivity.
+  - (*Flet*) simpl_rep_full. case_in.
+    + erewrite H. apply fmla_rep_irrel.
+    + erewrite H. apply H0.
+  - (*Fif*) simpl_rep_full. erewrite H, H0, H1; reflexivity.
+  - (*Fmatch*)  
+    simpl_rep_full.
+    iter_match_gen Hvalsub Htmsub Hpatsub Hvalsub.
+    iter_match_gen Hvalf Htmt Hpatt Hvalf.
+    clear n. induction ps; simpl; intros; try reflexivity.
+    destruct a as[p1 t1]; simpl in *.
+    rewrite H with (Htyt:=Hvalf) at 1.
+    rewrite match_val_single_irrel with(Hval2:=Forall_inv Hpatt).
+    simpl.
+    inversion H0; subst. inversion Htmt; subst.
+    inversion Hpatt; subst.
+    destruct (match_val_single gamma_valid pd vt v p1 (Forall_inv Hpatt)
+    (term_rep gamma_valid pd vt pf vv tm v Hvalf)) eqn : Hmatch; auto.
+    destruct (existsb _ _); auto.
+    apply fmla_rep_irrel.
+Qed.
+
+Definition replace_fmla_f_rep {gamma: context} 
+(gamma_valid: valid_context gamma)
+(fmla_o fmla_n: formula)
+(Hty1: formula_typed gamma fmla_o)
+(Hty2: formula_typed gamma fmla_n)
+(pd: pi_dom) (pf: pi_funpred gamma_valid pd)
+(vt: val_typevar)
+(Hrep: forall (vv: val_vars pd vt) Hty1 Hty2,
+    formula_rep gamma_valid pd vt pf vv fmla_o Hty1 =
+    formula_rep gamma_valid pd vt pf vv fmla_n Hty2)
+(f: formula) :=
+proj_fmla (replace_fmla_rep gamma_valid fmla_o fmla_n Hty1 Hty2
+  pd pf vt Hrep) f.
